theories/twoLockMSQ_concurrent_spec.v
@@ -184,10 +184,30 @@ Definition TokBefore (g : Qgnames) := own g.(γ_Before) (Excl ()).
 Definition TokAfter (g : Qgnames) := own g.(γ_After) (Excl ()).
 Definition TokUpdated (g : Qgnames) := ((TokBefore g) ∗ (TokAfter g))%I.
 
-Definition queue_invariant (l_head l_tail : loc) (Q_γ : Qgnames) : iProp Σ :=
-	∃ xs xs_rest xs_old (x_head x_tail: (loc * val * loc)),
+Fixpoint All {A} (xs : list A) (f : A -> iProp Σ) : iProp Σ :=
+	match xs with
+	| [] => True
+	| x :: xs' => f x ∗ All xs' f
+	end.
+
+Lemma All_split {A} : forall (xs_1 xs_2 : list A) f,
+	All (xs_1 ++ xs_2) f ∗-∗ All xs_1 f ∗ All xs_2 f.
+Proof.
+	iIntros (xs_1).
+	iInduction (xs_1) as [| x xs'_1] "IH"; iIntros (xs_2 f).
+	- simpl. iSplit; first auto. iIntros "[_ H]". done.
+	- simpl. iSplit.
+	  + iIntros "[Hfx HAll]". iFrame. by iApply "IH".
+	  + iIntros "[[Hfx HAll1] HAll2]". iFrame. iApply "IH". iFrame.
+Qed.
+
+Definition queue_invariant (Ψ : val -> iProp Σ) (l_head l_tail : loc) (Q_γ : Qgnames) : iProp Σ :=
+	∃ xs_v, (* Abstract state *)
+	∃ xs xs_rest xs_old (x_head x_tail: (loc * val * loc)), (* Concrete state *)
 	⌜xs = xs_rest ++ [x_head] ++ xs_old⌝ ∗
 	isLL xs ∗
+	⌜proj_val xs_rest = wrap_some xs_v⌝ ∗
+	All xs_v Ψ ∗
 	(
 		(* Static *)
 		(
@@ -222,9 +242,13 @@ Definition queue_invariant (l_head l_tail : loc) (Q_γ : Qgnames) : iProp Σ :=
 		)
 	).
 
-Definition queue_invariant_simple (l_head l_tail : loc) (Q_γ : Qgnames) : iProp Σ :=
-	∃ xs xs_rest xs_old (x_head x_tail: (loc * val * loc)),
-	⌜xs = xs_rest ++ [x_head] ++ xs_old⌝ ∗ isLL xs ∗
+Definition queue_invariant_simple (Ψ : val -> iProp Σ) (l_head l_tail : loc) (Q_γ : Qgnames) : iProp Σ :=
+	∃ xs_v, (* Abstract state *)
+	∃ xs xs_rest xs_old (x_head x_tail: (loc * val * loc)), (* Concrete state *)
+	⌜xs = xs_rest ++ [x_head] ++ xs_old⌝ ∗
+	isLL xs ∗
+	⌜proj_val xs_rest = wrap_some xs_v⌝ ∗
+	All xs_v Ψ ∗
 	(
 		(
 			(l_head ↦ #(n_in x_head) ∗ ToknD Q_γ) ∨ 
@@ -242,46 +266,52 @@ Definition queue_invariant_simple (l_head l_tail : loc) (Q_γ : Qgnames) : iProp
 		)
 	).
 
-Lemma queue_invariant_equiv_simple : forall l_head l_tail Q_γ,
-	(queue_invariant l_head l_tail Q_γ) ∗-∗
-	(queue_invariant_simple l_head l_tail Q_γ).
+Lemma queue_invariant_equiv_simple : forall Ψ l_head l_tail Q_γ,
+	(queue_invariant Ψ l_head l_tail Q_γ) ∗-∗
+	(queue_invariant_simple Ψ l_head l_tail Q_γ).
 Proof.
-	iIntros (l_head l_tail Q_γ).
+	iIntros (Ψ l_head l_tail Q_γ).
 	iSplit.
-	- iIntros "(%xs & %xs_rest & %xs_old & %x_head & %x_tail & Hxs_split & HisLL_xs & [H_Static | [H_Enqueue | [H_Dequeue | H_Both]]])"; 
-	iExists xs, xs_rest, xs_old, x_head, x_tail; iFrame.
+	- iIntros "(%xs_v & %xs & %xs_rest & %xs_old & %x_head & %x_tail & Hxs_split & HisLL_xs & %Hconc_abst_eq & HAll & [H_Static | [H_Enqueue | [H_Dequeue | H_Both]]])"; 
+	iExists xs_v, xs, xs_rest, xs_old, x_head, x_tail; iFrame.
 	  + iDestruct "H_Static" as "(Hl_head & Hl_tail & HisLast & HTokne & HToknD & HTokUpdated)".
+	  	iSplit; first done.
 		iSplitL "Hl_head HToknD"; first (iLeft; iFrame).
 		iLeft. iFrame.
 	  + iDestruct "H_Enqueue" as "(Hl_head & Hl_tail & [[HisLast HTokAfter] | [HisSndLast HAfter]] & HToke & HToknD)".
-	    * iSplitL "Hl_head HToknD"; first (iLeft; iFrame). 
+	    * iSplit; first done.
+		  iSplitL "Hl_head HToknD"; first (iLeft; iFrame). 
 		  iRight. iFrame. iLeft. iFrame.
-		* iSplitL "Hl_head HToknD"; first (iLeft; iFrame). 
+		* iSplit; first done.
+		  iSplitL "Hl_head HToknD"; first (iLeft; iFrame). 
 		  iRight. iFrame. iRight. iFrame.
 	  + iDestruct "H_Dequeue" as "(Hl_head & Hl_tail & HisLast & HTokne & HTokD & HTokUpdated)".
+	    iSplit; first done.
 		iSplitL "Hl_head HTokD"; first (iRight; iFrame).
 		iLeft. iFrame.
 	  + iDestruct "H_Both" as "(Hl_head & Hl_tail & [[HisLast HTokAfter] | [HisSndLast HAfter]] & HToke & HTokD)".
-	    * iSplitL "Hl_head HTokD"; first (iRight; iFrame). 
+	    * iSplit; first done.
+		  iSplitL "Hl_head HTokD"; first (iRight; iFrame). 
 		  iRight. iFrame. iLeft. iFrame.
-		* iSplitL "Hl_head HTokD"; first (iRight; iFrame). 
+		* iSplit; first done.
+		  iSplitL "Hl_head HTokD"; first (iRight; iFrame). 
 		  iRight. iFrame. iRight. iFrame.
-	- iIntros "(%xs & %xs_rest & %xs_old & %x_head & %x_tail & Hxs_split & HisLL_xs & [[Hl_head HToknD] | [Hl_head HTokD]] & [(Hl_tail & HisLast & HToknE & HTokUpdated) | (Hl_tail & HTokE & [[HisLast HTokBefore] | [HisSndLast HTokAfter]])])";
-	iExists xs, xs_rest, xs_old, x_head, x_tail; eauto 10 with iFrame.
+	- iIntros "(%xs_v & %xs & %xs_rest & %xs_old & %x_head & %x_tail & Hxs_split & HisLL_xs & %Hconc_abst_eq & HAll & [[Hl_head HToknD] | [Hl_head HTokD]] & [(Hl_tail & HisLast & HToknE & HTokUpdated) | (Hl_tail & HTokE & [[HisLast HTokBefore] | [HisSndLast HTokAfter]])])";
+	iExists xs_v, xs, xs_rest, xs_old, x_head, x_tail; eauto 10 with iFrame.
 Qed.
 
-Definition is_queue (q : val) (Q_γ: Qgnames) : iProp Σ :=
+Definition is_queue (Ψ : val -> iProp Σ) (q : val) (Q_γ: Qgnames) : iProp Σ :=
 	∃ head tail : loc, ∃ H_lock T_lock : val,
 	∃ l : loc , ⌜q = #l⌝ ∗
 		l ↦□ ((#head, #tail), (H_lock, T_lock)) ∗
-		inv N (queue_invariant head tail Q_γ) ∗
+		inv N (queue_invariant Ψ head tail Q_γ) ∗
 		is_lock Q_γ.(γ_Hlock) H_lock (TokD Q_γ) ∗
 		is_lock Q_γ.(γ_Tlock) T_lock (TokE Q_γ).
 
-Lemma initialize_spec :
+Lemma initialize_spec (Ψ : val -> iProp Σ):
 	{{{ True }}}
 		initialize #()
-	{{{ v Q_γ, RET v; is_queue v Q_γ}}}.
+	{{{ v Q_γ, RET v; is_queue Ψ v Q_γ}}}.
 Proof.
 	iIntros (Φ) "_ HΦ".
 	wp_lam.
@@ -314,9 +344,9 @@ Proof.
 							γ_Before := γ_Before;
 							γ_After := γ_After
 					|}).
-	iMod (inv_alloc N _ (queue_invariant l_head l_tail Queue_gnames) with "[Hl_head Hl_tail Hl_1_in Hl_1_out Hγ_nE Hγ_nD Hγ_Before Hγ_After]") as "#HqueueInv".
+	iMod (inv_alloc N _ (queue_invariant Ψ l_head l_tail Queue_gnames) with "[Hl_head Hl_tail Hl_1_in Hl_1_out Hγ_nE Hγ_nD Hγ_Before Hγ_After]") as "#HqueueInv".
 	{
-		iNext. iExists [(l_1_in, NONEV, l_1_out)], [], [], (l_1_in, NONEV, l_1_out), (l_1_in, NONEV, l_1_out). cbn. iSplitR; first done. iSplitL "Hl_1_in Hl_1_out"; first auto.
+		iNext. iExists [], [(l_1_in, NONEV, l_1_out)], [], [], (l_1_in, NONEV, l_1_out), (l_1_in, NONEV, l_1_out). cbn. iSplit; first done. iSplitL "Hl_1_in Hl_1_out"; first auto. do 2 (iSplit; first done).
 		iLeft. iFrame. iPureIntro. by exists [].
 	}
 	wp_alloc l_queue as "Hl_queue".
@@ -327,13 +357,13 @@ Proof.
 	by repeat iSplit.
 Qed.
 
-Lemma enqueue_spec Q (v : val) (qg : Qgnames) :
-	{{{ is_queue Q qg }}}
-		enqueue Q v 
-	{{{w, RET w; True}}}.
+Lemma enqueue_spec Q Ψ (v : val) (qg : Qgnames) :
+	{{{ is_queue Ψ Q qg ∗ Ψ v }}}
+		enqueue Q v
+	{{{ w, RET w; True }}}.
 Proof.
-	iIntros (Φ) "(%l_head & %l_tail & %H_lock & %T_lock & %l_queue & -> &
-				 #Hl_queue & #H_queue_inv & #H_hlock & #H_tlock) HΦ".
+	iIntros (Φ) "[(%l_head & %l_tail & %H_lock & %T_lock & %l_queue & -> &
+				 #Hl_queue & #H_queue_inv & #H_hlock & #H_tlock) HΨ_v] HΦ".
 	wp_lam.
 	wp_let.
 	wp_pures.
@@ -355,21 +385,21 @@ Proof.
 	wp_bind (! #l_tail)%E.
 	(* Open in Static / Dequeue *)
 	iInv "H_queue_inv" as "H_queue_inv_open".
-	iPoseProof (queue_invariant_equiv_simple with "H_queue_inv_open") as "H_queue_inv_open".
-	iDestruct "H_queue_inv_open" as "(%xs & %xs_rest & %xs_old & %x_head & %x_tail & >%H_eq_xs & HisLL_xs & H_head & [ ( [Hl_tail1 Hl_tail2] & >[%xs_fromtail %H_isLast] & HToknE & HTokUpdated ) | (_ & >HTokE2 & _) ])"; last by iCombine "HTokE HTokE2" gives "%H". (* Impossible: TokE *)
+	iPoseProof (queue_invariant_equiv_simple Ψ l_head l_tail qg with "H_queue_inv_open") as "H_queue_inv_open".
+	iDestruct "H_queue_inv_open" as "(%xs_v & %xs & %xs_rest & %xs_old & %x_head & %x_tail & >%H_eq_xs & HisLL_xs & >%Hconc_abst_eq & HAll_xs & H_head & [ ( [Hl_tail1 Hl_tail2] & >[%xs_fromtail %H_isLast] & HToknE & HTokUpdated ) | (_ & >HTokE2 & _) ])"; last by iCombine "HTokE HTokE2" gives "%H". (* Impossible: TokE *)
 	wp_load.
 	iModIntro.
 	iPoseProof (isLL_and_chain with "HisLL_xs") as "[HisLL_xs #HisLL_chain_xs]".
 	iPoseProof (isLL_chain_node [] x_tail xs_fromtail with "[HisLL_chain_xs]") as "#Hx_tail"; first by rewrite H_isLast.
 	iDestruct "HTokUpdated" as "[HTokBefore HTokAfter]".
 	(* Close in Enqueue / Both : Before *)
-	iSplitL "H_head Hl_tail1 HTokE HTokBefore HisLL_xs".
+	iSplitL "H_head Hl_tail1 HTokE HTokBefore HisLL_xs HAll_xs".
 	{
 		iNext.
 		iApply queue_invariant_equiv_simple.
-		iExists xs, xs_rest, xs_old, x_head, x_tail.
+		iExists xs_v, xs, xs_rest, xs_old, x_head, x_tail.
 		iFrame.
-		iSplitR; first done.
+		do 2 (iSplit; first done).
 		iRight.
 		iFrame.
 		iLeft.
@@ -381,8 +411,8 @@ Proof.
 	wp_bind (#(n_out x_tail) <- #l_new_in)%E.
 	(* Open in Enqueue / Both : Before *)
 	iInv "H_queue_inv" as "H_queue_inv_open".
-	iPoseProof (queue_invariant_equiv_simple with "H_queue_inv_open") as "H_queue_inv_open".
-	iDestruct "H_queue_inv_open" as "(%xs_2 & %xs_rest_2 & %xs_old_2 & %x_head_2 & %x_tail_2 & >%H_eq_xs_2 & HisLL_xs_2 & H_head & [ ( _ & _ & >HToknE2 & _ ) | (>Hl_tail1 & HTokE & [[>[%xs_fromtail_2 %H_isLast_2] HTokBefore] | [_ >HTokAfter2]]) ])"; 
+	iPoseProof (queue_invariant_equiv_simple Ψ l_head l_tail qg with "H_queue_inv_open") as "H_queue_inv_open".
+	iDestruct "H_queue_inv_open" as "(%xs_v_2 & %xs_2 & %xs_rest_2 & %xs_old_2 & %x_head_2 & %x_tail_2 & >%H_eq_xs_2 & HisLL_xs_2 & >%Hconc_abst_eq_2 & HAll_xs_2 & H_head & [ ( _ & _ & >HToknE2 & _ ) | (>Hl_tail1 & HTokE & [[>[%xs_fromtail_2 %H_isLast_2] HTokBefore] | [_ >HTokAfter2]]) ])"; 
 	[ by iCombine "HToknE HToknE2" gives "%H" | | (* Impossible: ToknE *)
 	  by iCombine "HTokAfter HTokAfter2" gives "%H" ]. (* Impossible: TokAfter *)
 	iCombine "Hl_tail1 Hl_tail2" as "Hl_tail" gives "[_ %Htail_eq]".
@@ -406,13 +436,14 @@ Proof.
 	}
 	iPoseProof (isLL_and_chain with "HisLL_xs_new") as "[HisLL_xs_new #HisLL_chain_xs_new]".
 	(* Close in Enqueue / Both: After *)
-	iSplitL "H_head Hl_tail1 HTokE HTokAfter HisLL_xs_new".
+	iSplitL "H_head Hl_tail1 HTokE HTokAfter HisLL_xs_new HAll_xs_2 HΨ_v".
 	{
 		iNext.
 		iApply queue_invariant_equiv_simple.
-		iExists xs_new, (x_new :: xs_rest_2), xs_old_2, x_head_2, x_tail.
-		iSplitR. { iPureIntro. unfold xs_new. cbn. rewrite H_eq_xs_2. auto. }
+		iExists (v :: xs_v_2), xs_new, (x_new :: xs_rest_2), xs_old_2, x_head_2, x_tail.
+		iSplit. { iPureIntro. unfold xs_new. cbn. rewrite H_eq_xs_2. auto. }
 		iFrame.
+		iSplit. { iPureIntro. simpl. f_equal. done. }
 		iRight.
 		iFrame.
 		iRight.
@@ -427,8 +458,8 @@ Proof.
 	wp_bind (#l_tail <- #l_new_in)%E.
 	(* Open in Enqueue / Both : After *)
 	iInv "H_queue_inv" as "H_queue_inv_open".
-	iPoseProof (queue_invariant_equiv_simple with "H_queue_inv_open") as "H_queue_inv_open".
-	iDestruct "H_queue_inv_open" as "(%xs_3 & %xs_rest_3 & %xs_old_3 & %x_head_3 & %x_tail_3 & >%H_eq_xs_3 & HisLL_xs_3 & H_head & [ ( _ & _ & >HToknE2 & _ ) | (>Hl_tail1 & HTokE & [[_ >HTokBefore2] | [>(%x_new_2 & %xs_fromtail_3 & %H_isSndLast) HTokAfter]])])"; 
+	iPoseProof (queue_invariant_equiv_simple Ψ l_head l_tail qg with "H_queue_inv_open") as "H_queue_inv_open".
+	iDestruct "H_queue_inv_open" as "(%xs_v_3 & %xs_3 & %xs_rest_3 & %xs_old_3 & %x_head_3 & %x_tail_3 & >%H_eq_xs_3 & HisLL_xs_3 & >%Hconc_abst_eq_3 & HAll_xs_3 & H_head & [ ( _ & _ & >HToknE2 & _ ) | (>Hl_tail1 & HTokE & [[_ >HTokBefore2] | [>(%x_new_2 & %xs_fromtail_3 & %H_isSndLast) HTokAfter]])])"; 
 	[ by iCombine "HToknE HToknE2" gives "%H" | (* Impossible: ToknE *)
 	  by iCombine "HTokBefore HTokBefore2" gives "%H" | ]. (* Impossible: TokBefore *)
 	iCombine "Hl_tail1 Hl_tail2" as "Hl_tail" gives "[_ %Htail_eq2]".
@@ -455,9 +486,10 @@ Proof.
 	{
 		iNext.
 		iApply queue_invariant_equiv_simple.
-		iExists xs_3, xs_rest_3, xs_old_3, x_head_3, x_new.
-		iSplitR; first done.
+		iExists xs_v_3, xs_3, xs_rest_3, xs_old_3, x_head_3, x_new.
+		iSplit; first done.
 		iFrame.
+		iSplit; first done.
 		iLeft.
 		iFrame.
 		by iExists (x_tail :: xs_fromtail_3).
@@ -469,10 +501,10 @@ Proof.
 	done.
 Qed.
 
-Lemma dequeue_spec Q (qg : Qgnames) : 
-	{{{ is_queue Q qg}}} 
+Lemma dequeue_spec Q Ψ (qg : Qgnames) : 
+	{{{ is_queue Ψ Q qg }}} 
 		dequeue Q 
-	{{{v, RET v; True}}}.
+	{{{ v, RET v; ⌜v = NONEV⌝ ∨ (∃ x_v, ⌜v = SOMEV x_v⌝ ∗ Ψ x_v) }}}.
 Proof.
 	iIntros (Φ) "(%l_head & %l_tail & %H_lock & %T_lock & %l_queue & -> &
 				 #Hl_queue & #H_queue_inv & #H_hlock & #H_tlock) HΦ".
@@ -487,19 +519,19 @@ Proof.
 	wp_bind (! #l_head)%E.
 	(* Open in Static / Enqueue *)
 	iInv "H_queue_inv" as "H_queue_inv_open".
-	iPoseProof (queue_invariant_equiv_simple with "H_queue_inv_open") as "H_queue_inv_open".
-	iDestruct "H_queue_inv_open" as "(%xs & %xs_rest & %xs_old & %x_head & %x_tail & >%H_eq_xs & H_isLL_xs & [ [Hl_head HToknD] | [Hl_head >HTokD2] ] & H_tail)"; 
+	iPoseProof (queue_invariant_equiv_simple Ψ l_head l_tail qg with "H_queue_inv_open") as "H_queue_inv_open".
+	iDestruct "H_queue_inv_open" as "(%xs_v & %xs & %xs_rest & %xs_old & %x_head & %x_tail & >%H_eq_xs & H_isLL_xs & >%Hconc_abst_eq & HAll_xs & [ [Hl_head HToknD] | [Hl_head >HTokD2] ] & H_tail)"; 
 	last by iCombine "HTokD HTokD2" gives "%H". (* Impossible: TokD*)
 	wp_load.
 	iModIntro.
 	iDestruct "Hl_head" as "[Hl_head1 Hl_head2]".
 	iPoseProof (isLL_and_chain with "H_isLL_xs") as "[H_isLL_xs #H_isLL_chain_xs_1]".
 	(* Close in Dequeue / Both *)
-	iSplitL "Hl_head2 HTokD H_tail H_isLL_xs".
+	iSplitL "Hl_head2 HTokD H_tail H_isLL_xs HAll_xs".
 	{
 		iNext. iApply queue_invariant_equiv_simple.
-		iExists xs, xs_rest, xs_old, x_head, x_tail. iFrame.
-		iSplitR; first done. iRight. done.
+		iExists xs_v, xs, xs_rest, xs_old, x_head, x_tail. iFrame.
+		do 2 (iSplit; first done). iRight. done.
 	}
 	wp_let.
 	subst.
@@ -509,8 +541,8 @@ Proof.
 	wp_bind (! #(n_out x_head))%E.
 	(* Open in Dequeue / Both *)
 	iInv "H_queue_inv" as "H_queue_inv_open".
-	iPoseProof (queue_invariant_equiv_simple with "H_queue_inv_open") as "H_queue_inv_open".
-	iDestruct "H_queue_inv_open" as "(%xs_2 & %xs_rest_2 & %xs_old_2 & %x_head_2 & %x_tail_2 & >%H_eq_xs_2 & H_isLL_xs_2 & [ [Hl_head >HToknD2] | [>Hl_head2 HTokD] ] & H_tail)";
+	iPoseProof (queue_invariant_equiv_simple Ψ l_head l_tail qg with "H_queue_inv_open") as "H_queue_inv_open".
+	iDestruct "H_queue_inv_open" as "(%xs_v_2 & %xs_2 & %xs_rest_2 & %xs_old_2 & %x_head_2 & %x_tail_2 & >%H_eq_xs_2 & H_isLL_xs_2 & >%Hconc_abst_eq_2 & HAll_xs_2 & [ [Hl_head >HToknD2] | [>Hl_head2 HTokD] ] & H_tail)";
 	first by iCombine "HToknD HToknD2" gives "%H". (* Impossible: ToknD*)
 	iPoseProof (isLL_and_chain with "H_isLL_xs_2") as "[H_isLL_xs_2 #HisLL_chain_xs_2]".
 	iCombine "Hl_head1 Hl_head2" as "Hl_head" gives "[_ %Hhead_eq2]".
@@ -531,8 +563,8 @@ Proof.
 	  iSplitL "Hl_head HToknD H_tail H_x_head_out".
 	  {
 		iNext. iApply queue_invariant_equiv_simple.
-		iExists ([] ++ [x_head] ++ xs_old_2), [], xs_old_2, x_head, x_tail_2.
-		iFrame. iSplitR; first done. iSplitR; first done. iLeft. iFrame.
+		iExists [], ([] ++ [x_head] ++ xs_old_2), [], xs_old_2, x_head, x_tail_2.
+		iFrame. do 3 (iSplit; first done). iLeft. iFrame.
 		rewrite dfrac_op_own. rewrite Qp.half_half. done.
 	  }
 	  wp_let.
@@ -544,7 +576,7 @@ Proof.
 	  wp_seq.
 	  iModIntro.
 	  iApply "HΦ".
-	  done.
+	  by iLeft.
 	- (* Queue is non-empty*)
 	  destruct (exists_first (x_tail_2_2 :: xs_rest_2')) as [x_head_next [xs_rest_2'' Hxs_rest_eq]]; first done.
 	  rewrite Hxs_rest_eq.
@@ -562,11 +594,11 @@ Proof.
 	  iModIntro.
 	  iDestruct "Hl_head" as "[Hl_head1 Hl_head2]".
 	  (* Close in Dequeue / Both *)
-	  iSplitL "Hl_head2 H_isLL_xs_2 H_tail HTokD".
+	  iSplitL "Hl_head2 H_isLL_xs_2 H_tail HTokD HAll_xs_2".
 	  {
 		iNext. iApply queue_invariant_equiv_simple.
-		iExists ((xs_rest_2'' ++ [x_head_next]) ++ [x_head] ++ xs_old_2), (xs_rest_2'' ++ [x_head_next]), xs_old_2, x_head, x_tail_2.
-		iFrame. iSplitR; first done. iRight. done.
+		iExists xs_v_2, ((xs_rest_2'' ++ [x_head_next]) ++ [x_head] ++ xs_old_2), (xs_rest_2'' ++ [x_head_next]), xs_old_2, x_head, x_tail_2.
+		iFrame. iSplit; first done. iSplit; first by rewrite <- Hxs_rest_eq.  iRight. done.
 	  }
 	  wp_let.
 	  wp_pures.
@@ -575,38 +607,53 @@ Proof.
 	  wp_load.
 	  wp_pures.
 	  wp_bind (#l_head <- #(n_in x_head_next))%E.
+	  (* Open in Dequeue / Both *)
 	  iInv "H_queue_inv" as "H_queue_inv_open".
-	  iPoseProof (queue_invariant_equiv_simple with "H_queue_inv_open") as "H_queue_inv_open".
-	  iDestruct "H_queue_inv_open" as "(%xs_3 & %xs_rest_3 & %xs_old_3 & %x_head_3 & %x_tail_3 & >%H_eq_xs_3 & H_isLL_xs_3 & [ [Hl_head >HToknD2] | [>Hl_head2 HTokD] ] & H_tail)";
+	  iPoseProof (queue_invariant_equiv_simple Ψ l_head l_tail qg with "H_queue_inv_open") as "H_queue_inv_open".
+	  iDestruct "H_queue_inv_open" as "(%xs_v_3 & %xs_3 & %xs_rest_3 & %xs_old_3 & %x_head_3 & %x_tail_3 & >%H_eq_xs_3 & H_isLL_xs_3 & >%Hconc_abst_eq_3 & HAll_xs_3 & [ [Hl_head >HToknD2] | [>Hl_head2 HTokD] ] & H_tail)";
 	  first by iCombine "HToknD HToknD2" gives "%H". (* Impossible ToknD *)
 	  iCombine "Hl_head1 Hl_head2" as "Hl_head" gives "[_ %Hhead_eq3]".
 	  rewrite dfrac_op_own.
 	  rewrite Qp.half_half.
 	  wp_store.
 	  iModIntro.
-	  (* Close in Static / Enqueue *)
-	  iSplitL "Hl_head H_tail HToknD H_isLL_xs_3".
+	  iPoseProof (isLL_and_chain with "H_isLL_xs_3") as "[H_isLL_xs_3 #H_isLL_chain_xs_3]".
+	  iAssert (⌜x_head_3 = x_head⌝)%I as "->".
 	  {
-		iNext.
-		iPoseProof (isLL_and_chain with "H_isLL_xs_3") as "[H_isLL_xs_3 #H_isLL_chain_xs_3]".
-		subst.
-		iAssert (⌜x_head_3 = x_head⌝)%I as "->".
-		{
-			iApply (isLL_chain_agree x_head_3 x_head xs_rest_3 xs_old_3 xs_rest xs_old); by simplify_eq.
-		}
-		(* Sync up xs_rest_2 with xs_rest_3 *)
-		destruct xs_rest_3 as [|x_tail_3_2 xs_rest_3'].
-		- (* Impossible case. xs_rest_3 must contain at least one element. *)
-		  iDestruct "H_isLL_xs_3" as "[H_x_head_3_null _]".
-		  iCombine "H_x_head_3_null H_x_head_next_out" gives "[_ %Hcontra]".
-		  simplify_eq.
-		- destruct (exists_first (x_tail_3_2 :: xs_rest_3')) as [x_head_next_3 [xs_rest_3'' Hxs_rest_eq_3]]; first done.
-		  rewrite Hxs_rest_eq_3.
-		  rewrite <- app_assoc. rewrite <- app_assoc.
-		  iAssert (⌜x_head_next = x_head_next_3⌝)%I as "->"; first by iApply isLL_chain_agree_next.
-		  iApply queue_invariant_equiv_simple.
-		  iExists (xs_rest_3'' ++ [x_head_next_3] ++ [x_head] ++ xs_old_3), xs_rest_3'', ([x_head] ++ xs_old_3), x_head_next_3, x_tail_3.
-		  iFrame. iSplitR; first done. iLeft. iFrame.
+		iApply (isLL_chain_agree x_head_3 x_head xs_rest_3 xs_old_3 xs_rest xs_old); by simplify_eq.
+	  }
+	  subst.
+	  (* Sync up xs_rest_2 with xs_rest_3 *)
+	  destruct xs_rest_3 as [|x_tail_3_2 xs_rest_3'].
+	  { (* Impossible case. xs_rest_3 must contain at least one element. *)
+		iDestruct "H_isLL_xs_3" as "[H_x_head_3_null _]".
+		iCombine "H_x_head_3_null H_x_head_next_out" gives "[_ %Hcontra]".
+		simplify_eq.
+	  }
+	  destruct (exists_first (x_tail_3_2 :: xs_rest_3')) as [x_head_next_3 [xs_rest_3'' Hxs_rest_eq_3]]; first done.
+	  rewrite Hxs_rest_eq_3.
+	  rewrite <- app_assoc. rewrite <- app_assoc.
+	  iAssert (⌜x_head_next = x_head_next_3⌝)%I as "->"; first by iApply isLL_chain_agree_next.
+	  destruct xs_v_3 as [|x_v xs'_v_3]; 
+	  	first inversion Hconc_abst_eq_3. (* Impossible case. xs_v_3 must contain at least one element. *)
+	  destruct (exists_first (x_v :: xs'_v_3)) as [x_head_next_val [xs_val_rest Hxs_val_rest_eq]]; first done.
+	  rewrite Hxs_val_rest_eq in Hconc_abst_eq_3.
+	  rewrite Hxs_val_rest_eq.
+	  rewrite Hxs_rest_eq_3 in Hconc_abst_eq_3.
+	  rewrite (proj_val_split xs_rest_3'' [x_head_next_3]) in Hconc_abst_eq_3.
+	  rewrite (wrap_some_split xs_val_rest [x_head_next_val]) in Hconc_abst_eq_3.
+	  simpl in Hconc_abst_eq_3.
+	  apply (list_last_eq (proj_val xs_rest_3'') (wrap_some xs_val_rest) (n_val x_head_next_3) (InjRV x_head_next_val)) in Hconc_abst_eq_3 as [Hxs_rest_val_eq Hx_head_next_eq].
+	  iPoseProof (All_split with "HAll_xs_3") as "[HAll_xs_val_rest [Hx_head_next_val_Ψ _]]".
+	  (* Close in Static / Enqueue *)
+	  iSplitL "Hl_head H_tail HToknD H_isLL_xs_3 HAll_xs_val_rest".
+	  {
+		iNext. iApply queue_invariant_equiv_simple.
+		iExists xs_val_rest, (xs_rest_3'' ++ [x_head_next_3] ++ [x_head] ++ xs_old_3), xs_rest_3'', ([x_head] ++ xs_old_3), x_head_next_3, x_tail_3.
+		iFrame. iSplit; first done.
+		iSplit; first done.
+		iLeft.
+		iFrame.
 	  }
 	  wp_seq.
 	  wp_load.
@@ -616,7 +663,9 @@ Proof.
 	  wp_seq.
 	  iModIntro.
 	  iApply "HΦ".
-	  done.
+	  iRight.
+	  iExists x_head_next_val.
+	  by iSplit.
 Qed.
 
 End proofs.
