Tasks.md
@@ -30,16 +30,17 @@
   - [x] Change l_null to l_n+1
   - [x] Do proof sketch on paper
   - [x] Implement proof in Iris (Coq)
-  - [ ] Add a predicate that should hold of all elements in queue (see isBag)
+  - [x] Add a predicate that should hold of all elements in queue (see isBag)
   - [x] use {} and [] instead of i: 
 
 - [ ] Clean up proof of concurrent spec for M&S queue with locks in Coq
-- [ ] Clean up proof of Sequential spec for M&S queue with locks in Coq
+- [x] Clean up proof of Sequential spec for M&S queue with locks in Coq
 
 - [ ] Write about the sequential spec for two-lock M&S queue in the report
   - [ ] Mention how it can be used to track exact contents of queue
   - [ ] Can be used to prove a precise spec for sequential client used in testing.
 - [ ] Write about the concurrent spec for two-lock M&S queue in the report
   - [ ] Talk about adequacy as a reason for safety.
+  - [ ] Update spec to include the Ψ predicate.
 
 - [ ] State and prove correctness of lock-free M&S Queue
